Answersheet 12  - Yiwei Yang 2018533218

## 1.

Since $\left[E_{1} E _{2}: k\right]=\left[E_{1} E_{2}: L_{1}\right]\left[L_{2}: k\right]$, it suffices to show $\left[E_{1} E_{2}: E_{1}\right] \leq\left[E_{2}: k\right] .$ Let $\left\{e_{i}\right\}$ be a $k$ -basis of $E_{2}$. Since the $E_{j}$ 's are finite algebraic over $k, E_{1} E_{2}$ consists of polynomials in elements of $E_{2}$ with coefficients in $E_{1}$, so $E_{1} E_{2}$ is spanned by the $\left\{e_{i}\right\}$ over $E_{1}$ (but possibly with linear dependence relations). 



## 2.

### a.

First prove that the intersection is finite if it's non-empty.

By contradiction, suppose $\cap_{n \in N} A_{n}=\phi$. For each $x \in A_{1}$ let $f(x)$ be the least $n \in N$ such that $x \notin A_{n}$. Then $B=\left\{f(x): x \in A_{1}\right\}$ is a finite subset of $N$, so there exists $m \in N$ such that $\forall n \in B(m \geq n)$
For such an $m$, we have $\forall x \in A_{1}\left(x \notin A_{m}\right)$ because $\forall x \in A_{1}\left(x \notin A_{f(x)} \supset \cap_{j=f(x)}^{m} A_{j} \supset A_{m}\right)$. But
then $A_{m} \cap A_{1}=\phi$, contradicting $\phi \neq A_{m} \subset \cap_{j=1}^{m} A_{j} \subset A_{1}$.

Then prove that there's a bijection between profinite group of $A$ and extending sequence $A_n$ of finite primary groups belong  to $C_I$ is that $A_n$ be regular

Proof. Again, it is immediate that the condition is necessary. In fact, one needs only to make the obvious replacements in the proof of Theorem 1. Recall that $\sum \oplus$, the direct sum, should be replaced by $\sum^{\prime} \oplus$, the complete direct sum, and the group of type $p^{\infty}$ by the $p$ -adic group.

Denote by $A^{*}$ the (discrete) character group of $A .$ With an inverse sequence
$$
A_{1} \leftarrow A_{2} \leftarrow \cdots \leftarrow A_{n} \leftarrow \cdots
$$
there is associated in a natural way a (unique) direct sequence
$$
A_{1}^{*} \rightarrow A_{2}^{*} \rightarrow \cdots \rightarrow A_{n}^{*} \rightarrow \cdots
$$
which in turn gives rise to an inverse sequence
$$
A{1}^{* *} \leftarrow A_{2}^{* *} \leftarrow \cdots \leftarrow A_{n}^{* *} \leftarrow \cdots
$$
Together with the usual isomorphism between $A_{n}$ and $A_{n}^{* *},(1)$ and (3) form a commutative diagram and therefore have isomorphic limits. However, the limit of (3) is the character group of the limit of (2). Thus if $A_{n}$ is regular, the limit of (1) is determined by the groups alone and $A_{n} \in C_{I}$.

Now let $A_{n}$ be an extending sequence of finitely generated groups. Analogous to the $p$ -rank of a sequence, the torsion free rank of the sequence $A_{n}$ is defined as the limit of the torsion free ranks of the groups $A_{n}, r_{0}=\lim _{n \rightarrow \infty} r_{0}\left(A_{n}\right) .$ The question of whether or not $A_{n}$ is contained in $\mathrm{C}_{I}$ depends to a large degree on whether $r_{0}$ is finite or not; consequently, the two cases are distinguished.

Reference: Hill, Paul. "Limits of sequences of finitely generated abelian groups." *Proceedings of the American Mathematical Society*12.6 (1961): 946-950.

### b.

The elements of $\hat{\mathbb{Z}}$ have very explicit descriptions in terms of compatible sequences $\left(x_{i}\right)_{i \in \mathbb{N}}$ where each $x_{i} \in \mathbb{Z} / i \mathbb{Z}$. Note that $\hat{\mathbb{Z}}=\prod_{p} \mathbb{Z}_{p}$. 

Show that the equation $x^{2}=2$ has a solution in $\mathbb{Z}_{7}$ where: $\mathbb{Z}_{7}={^\lim_\longleftarrow } A_{n},\left(A_{n}=\mathbb{Z} / 7^{n} \mathbb{Z}\right)$

Consider the polynomial 𝑓(𝑥)=𝑥2−2f(x)=x2−2, check that there is some 𝑎∈ℤ/7ℤa∈Z/7Z such that 𝑓(𝑎)=0f(a)=0 but 𝑓′(𝑎)≠0f′(a)≠0, and apply Hensel's Lemma.

Proof of Hensel's Lemma: If $f(X) \in \mathbf{Z}_{p}[X]$ and $a \in \mathbf{Z}_{p}$ satisfies: $f(a)≡0\ mod\ p$, $f′(a)̸≡0\ mod\ p$. then there is a unique $\alpha \in \mathbf{Z}_{p}$ such that $f(\alpha)=0$ in $\mathbf{Z}_{p}$ and $\alpha \equiv a \bmod p .$

 We will prove by induction that for each $n \geq 1$ there is an $a_{n} \in \mathbf{Z}_{p}$ such that
- $f\left(a_{n}\right) \equiv 0 \bmod p^{n}$
- $a_{n} \equiv a \bmod p$.

Since $f\left(a_{n+1}\right) \equiv 0 \bmod p^{n+1} \Rightarrow f\left(a_{n+1}\right) \equiv 0 \bmod p^{n}$, each root of $f(X) \bmod p^{n+1}$ reduces
to a root of $f(X) \bmod p^{n}$. By the inductive hypothesis there is a root $a_{n} \bmod p^{n}$, so we seek a $p$ -adic integer $a_{n+1}$ such that $a_{n+1} \equiv a_{n} \bmod p^{n}$ and $f\left(a_{n+1}\right) \equiv 0 \bmod p^{n+1}$. Writing $a_{n+1}=a_{n}+p^{n} t_{n}$
for some $t_{n} \in \mathbf{Z}_{p}$ to be determined, can we make $f\left(a_{n}+p^{n} t_{n}\right) \equiv 0 \bmod p^{n+1} ?$
To compute $f\left(a_{n}+p^{n} t_{n}\right) \bmod p^{n+1}$, we use a polynomial identity:
$(2.1)$
$$
f(X+Y)=f(X)+f^{\prime}(X) Y+g(X, Y) Y^{2}
$$
for some polynomial $g(X, Y) \in \mathbf{Z}_{p}[X, Y] .$ This formula comes from isolating the first two terms in the binomial theorem: writing $f(X)=\sum_{i=0}^{d} c_{i} X^{i}$ we have
$$
f(X+Y)=\sum_{i=0}^{d} c_{i}(X+Y)^{i}=c_{0}+\sum_{i=1}^{d} c_{i}\left(X^{i}+i X^{i-1} Y+g_{i}(X, Y) Y^{2}\right)
$$
where $g_{i}(X, Y) \in \mathbf{Z}[X, Y] .$ Thus
$$
f(X+Y)=\sum_{i=0}^{d} c_{i} X^{i}+\sum_{i=1}^{d} i c_{i} X^{i-1} Y+\sum_{i=1}^{d} g_{i}(X, Y) Y^{2}=f(X)+f^{\prime}(X) Y+g(X, Y) Y^{2}
$$
where $g(X, Y)=\sum_{i=1}^{d} c_{i} g_{i}(X, Y) \in \mathbf{Z}_{p}[X, Y] .$ This gives us the desired identity. ${ }^{1}$ To make $(2.1)$ numerical, for all $x$ and $y$ in $\mathbf{Z}_{p}$ the number $z:=g(x, y)$ is in $\mathbf{Z}_{p}$, so
$(2.2)$
$x, y \in \mathbf{Z}_{p} \Longrightarrow F(x+y)=f(x)+f^{\prime}(x) y+z y^{2}$, where $z \in \mathbf{Z}_{p}$
In this formula set $x=a_{n}$ and $y=p^{n} t_{n}$ :
$(2.3)$
$f\left(a_{n}+p^{n} t_{n}\right)=f\left(a_{n}\right)+f^{\prime}\left(a_{n}\right) p^{n} t_{n}+z p^{2 n} t_{n}^{2} \equiv f\left(a_{n}\right)+f^{\prime}\left(a_{n}\right) p^{n} t_{n} \bmod p^{n+1}$
since $2 n \geq n+1 .$ In $f^{\prime}\left(a_{n}\right) p^{n} t_{n} \bmod p^{n+1}$, the factors $f^{\prime}\left(a_{n}\right)$ and $t_{n}$ only matter mod $p$ since there is already a factor of $p^{n}$ and the modulus is $p^{n+1}$. Recalling that $a_{n} \equiv a \bmod p$ we get $f^{\prime}\left(a_{n}\right) p^{n} t_{n} \equiv f^{\prime}(a) p^{n} t_{n} \bmod p^{n+1}$. Therefore from (2.3),
$$
\begin{aligned}
f\left(a_{n}+p^{n} t_{n}\right) \equiv 0 \bmod p^{n+1} & \Longleftrightarrow f\left(a_{n}\right)+f^{\prime}(a) p^{n} t_{n} \equiv 0 \bmod p^{n+1} \\
& \Longleftrightarrow f^{\prime}(a) t_{n} \equiv-f\left(a_{n}\right) / p^{n} \bmod p
\end{aligned}
$$
where the ratio $f\left(a_{n}\right) / p^{n}$ is in $\mathbf{Z}_{p}$ since we assumed that $f\left(a_{n}\right) \equiv 0 \bmod p^{n}$. There is a solution for $t_{n}$ in the congruence $\bmod p$ since we assumed that $f^{\prime}(a) \not \equiv 0 \bmod p$.

Armed with this choice of $t_{n}$ and setting $a_{n+1}=a_{n}+p^{n} t_{n}$, we have $f\left(a_{n+1}\right) \equiv 0 \bmod p^{n+1}$ and $a_{n+1} \equiv a_{n} \bmod p^{n}$, so in particular $a_{n+1} \equiv a \bmod p .$ This completes the induction. Starting with $a_{1}=a$, our inductive argument has constructed a sequence $a_{1}, a_{2}, a_{3}, \ldots$ in $\mathbf{Z}_{p}$ such that $f\left(a_{n}\right) \equiv 0 \bmod p^{n}$ and $a_{n+1} \equiv a_{n} \bmod p^{n}$ for all $n .$ The second condition, $a_{n+1} \equiv a_{n} \bmod p^{n}$, implies that $\left\{a_{n}\right\}$ is a Cauchy sequence in $\mathbf{Z}_{p} .$ Let $\alpha$ be its limit in $\mathbf{Z}_{p} .$ We want to show $f(\alpha)=0$ and $\alpha \equiv a \bmod p$ From $a_{n+1} \equiv a_{n} \bmod p^{n}$ for all $n$ we get $a_{m} \equiv a_{n} \bmod p^{n}$ for all $m>n$, so $\alpha \equiv a_{n} \bmod p^{n}$
by letting $m \rightarrow \infty .$ At $n=1$ we get $\alpha \equiv a \bmod p .$ For general $n$,
$$
\alpha \equiv a_{n} \bmod p^{n} \Longrightarrow f(\alpha) \equiv f\left(a_{n}\right) \equiv 0 \bmod p^{n} \Longrightarrow|f(\alpha)|_{p} \leq \frac{1}{p^{n}}
$$
Since this estimate holds for all $n, f(\alpha)=0$.

It remains to show $\alpha$ is the unique root of $f(X)$ in $\mathbf{Z}_{p}$ that is congruent to $a \bmod p$. Suppose $f(\beta)=0$ and $\beta \equiv a \bmod p$. To show $\beta=\alpha$ we will show $\beta \equiv \alpha \bmod p^{n}$ for all $n$. The case $n=1$ is clear since $\alpha$ and $\beta$ are both congruent to $a \bmod p$. Suppose $n \geq 1$ and we know that $\beta \equiv \alpha \bmod p^{n}$. Then $\beta=\alpha+p^{n} \gamma_{n}$ with $\gamma_{n} \in \mathbf{Z}_{p}$, so a calculation similar to implies
$$
f(\beta)=f\left(\alpha+p^{n} \gamma_{n}\right) \equiv f(\alpha)+f^{\prime}(\alpha) p^{n} \gamma_{n} \bmod p^{n+1}
$$
Both $\alpha$ and $\beta$ are roots of $f(X)$, so $0 \equiv f^{\prime}(\alpha) p^{n} \gamma_{n} \bmod p^{n+1}$. Thus $f^{\prime}(\alpha) \gamma_{n} \equiv 0 \bmod p$.
Since $f^{\prime}(\alpha) \equiv f^{\prime}(a) \not \equiv 0 \bmod p$, we have $\gamma_{n} \equiv 0 \bmod p$, which implies $\beta \equiv \alpha \bmod p^{n+1}$.

## 3.

Let $f\in F[X]$ be the irreducible polynomial of $\alpha.$ The degree of $f$ is odd. Let $f=X^{d}+f_{d-1} x^{d-1}+\cdots+f_{0}, f_{i} \in F$. Then. we have $\alpha^{d}+f_{d-1} \alpha^{d-1}+\cdots+f_{0}=0$. Seperate the even and odd powers. We can see that there exists $h, g \in F[X]$ with $h$ monic, such that, $\alpha h\left(\alpha^{2}\right)=g\left(\alpha^{2}\right)$. This shows that, $\alpha \in F\left(\alpha^{2}\right)$ and hence $F(\alpha)=F\left(\alpha^{2}\right)$.

## 4.

Proof. There is an obvious embedding of $Y$ into $\varliminf_{i}\left(\varphi_{i}(Y)\right)$. Since $Y$ is compact and Hausdorff, the previous corollary implies that the induced mapping of $Y$ to $\lim \left(\varphi_{i}(Y)\right)$ is onto, and by uniqueness this mapping is the afore mentioned embedding in (i). Thus we find that $$Y=\lim _{\underline{L}}\left(\varphi_{i}(Y)\right)$$
