Answer sheet 5 - Yiwei Yang 2018533218

## 1.
### a.
I'll show that $[SL_n(\R),SL_n(\R)]=SL_n(\R)$. that is to say $SL_n(\R)$ is perfect. Let $k$ be a field. $SL(n,k)$ is the special linear group over $k$.

First, elementary matrices of the first kind generate the special lineasr group over a field. The group of invertible $n*n$ matrices over $k$ with determinant equal to 1. Then $SL(n,k)$ is generated by elementary matrices of form $E_{i,j}$, where $\lambda \in K,1\leq i,j \leq n, i\neq j$. By useal Gauss-Jordan ellimination, the matrix $E_{i,j}(\lambda)$ has 1s on the diagonal, $\lambda$ in the $(ij) ^{th}$ position and 0 elsewhere.

Then for $n\geq 2$ number, for $i\neq j$ in the set $\{1,2,...n\}$ and $\lambda \in k$, let $e_{i j}(\lambda)$ be the matrix with $\lambda$ in the $(i j)^{t h}$ position and 0 elsewhere, $E_{i j}(\lambda)$ be termed elementary matrices and $\in SL_n{k} \forall i\neq j ,\lambda \in k$

1. If $n \geq 3$, every elementary matrix can be expressed as a commutator of two elementary matrices. In particular, it is the commutator of two elements of $S L_{n}(k)$.  
Pick $l \in\{1,2,3, \ldots, n\}$ different from $i, j$. Consider elements:
$g=E_{i l}(\lambda), \quad h=E_{l j}(1)$
Then, the commutator is given by:
$g h g^{-1} h^{-1}=E_{i l}(\lambda) E_{l j}(1) E_{i l}(-\lambda) E_{l j}(-1)$
Rewriting in terms of the $e_{i j}$ s:
$\left.\left.g h g^{-1} h^{-1}=\left(I+e_{i l}(\lambda)\right)\left(I+e_{l j}(1)\right)\left(I-e_{i l}(\lambda)\right)\right) I-e_{l j}(1)\right)$
Simplifying this yields:
$g h g^{-1} h^{-1}=\left(I+e_{i l}(\lambda)+e_{l j}(1)+e_{i j}(\lambda)\right)\left(I-e_{i l}(\lambda)-e_{l j}(1)+e_{i j}(\lambda)\right)$
Further simplification yields:
$g h g^{-1} h^{-1}=I+e_{i j}(\lambda)=E_{i j}(\lambda)$

2. If $n=2$, and $k$ has more than three elements, every elementary matrix can be expressed as a commutator of two elements of $S L_{n}(k)$.
If $k$ has more than three elements, there exists $\mu \in k$ such that $\mu$ is invertible and $\mu^{2} \neq 1$.
We need to prove that for any $\lambda$, the element $E_{12}(\lambda)$ (and analogously, the element $\left.E_{21}(\lambda)\right)$ is expressible as a commutator. Indeed, set:
$g=\left(\begin{array}{cc}\mu & 0 \\ 0 & \mu^{-1}\end{array}\right), \quad h=\left(\begin{array}{cc}1 & \frac {\lambda}{ \mu^{2}-1} \\ 0 & 1\end{array}\right)$.
A computation shows that the commutator of $g$ and $h$ is $E_{12}(\lambda) .$ A similar construction gives $E_{21}(\lambda)$ as a commutator.$\square$

### b.
 If $n=2$, we apply the commutator relation, $[\left(\begin{array}{cc}\mu & 0 \\ 0 & \mu^{-1}\end{array}\right),\left(\begin{array}{cc}1 & \tau \\ 0 & 1\end{array}\right)]=\left(\begin{array}{cc}1 & (\mu^2-1)\tau \\ 0 & 1\end{array}\right)$ but for any $\lambda \in k$, we have $\lambda = (\mu^2-1)\tau$. This can be solved for $\tau$ as long as there exists a unit $\mu\in k^{\text{x}}$ so that $\mu\neq\pm 1$. this only works with at least 3 elements in $k^{\text{x}}$. $\square$

## 2.
### a.
For $(\Z/n\Z,\text{x},\cdot  ),$ if $n$ is a composite number, then there are $1<a, b<n$ such that $a b=n$. Hence $a+n \mathbb{Z}$ and $b+n \mathbb{Z}$
are non-zero and their product is zero. So $\mathbb{Z} / n \mathbb{Z}$ has zero-divisors.

If $p$ is prime, then $p \mid a b$ if and only if either $p \mid a$ or $p \mid b$. Hence $\mathbb{Z} / p \mathbb{Z}$ is a unital (non-trivial) commutative ring without zero-divisors.

If $n=1,$ then $\mathbb{Z} / n \mathbb{Z}$ is the trivial ring which is not an integral domain (by the definition).

### b.
First, 1 plays the same role in multiplication as o does in addition: $1 \times a=a, 0+a=a$. They are called
the identity. (o is the additive identity in $\mathbb{Z}_{30}, 1$ is the multiplicative identity in $\mathbb{Z}_{31}^{\times}$ ).

Then look into $(\Z_{31})^*$ in detail. For $[1]$, it's clearly the multiplicative idnetity. For $[2]$, $[2]^5  \equiv 1 (mod\ 31)$, so order is 5. For $[3]$, $[3]^30 =[1]$ 

So 3 generates the whole group $\mathbb{Z}_{31}^{\times}$.$\square$

### c.
No integer solution.

It's a well known and pretty useful fact that the only possible remainders when a perfect
cube is divided by 9 are -1,0 and 1 (we can easily prove it using Euclid's division
lemma and then checking remainders of the first nine cubes).
That is, for an integer $n$ we have,
$n^{3} \equiv \pm 1(mod\ 9)$ when $n$ is not divisible by 3
and, $n^{3} \equiv 0(mod\ 9)$ when $n$ is divisible by 3.

Since, each of the cubes can only take any one of the values of -1,0 and $1,$ so the all
possible values of $x^{3}+y^{3}-z^{3}(mod\ 9)$ are -3,-2,-1,0,1,2 and 3, but $x^{3}+y^{3}-z^{3} \equiv 4$, which is contradiction.$\square$

## 3.
### a.

Denote $N=\bigcap_{g \in G} g H g^{-1}$ be the family of all normal subgroups of $G$ contained in $H$. The family is non-empty, since $1\subseteq H$ is a normal subgroup of $G$. We claim $N\ =\Sigma_{\lambda \in \Lambda}N_\lambda$, the group generated by all the $N_\lambda$'s, satisfied the conditions given. First, since $N_\lambda \subseteq H$ for each $\lambda \in \Lambda$, clearly we also have $N\subseteq H$. Every normal subgroup of $G$ contained in $H$ is one of the $N_\lambda$, which is by definition contained in $N$. Thus, since an element of $N$ is of the form $h_1,h_2...h_m$, where $h_n\in N_{\lambda_n}$ , for each $g\in G$ , we have $g(h_1h_2...h_n)g^{-1}=(gh_1g^{-1})(gh_2g^{-1})...(gh_ng^{-1})\subseteq N$, $N$ is a normal subgroup of $G$.

### b.

If $N$ is a normal subgroup of group $G$ and $n \in N$ then $g n g^{-1} \in N$ for every $g \in G$ or equivalently $[n] \subseteq N$ where $[n]:=\left\{g n g^{-1} \mid g \in G\right\}$ is the conjugacy class of $n$.
This tells us that:

$N$ is normal $\Leftrightarrow \forall g \in G, N=g N g^{-1}$

$
\begin{array}{l}
\Leftrightarrow \forall n \in N \forall g \in G \exists m_{n, g} \in N, n=g m_{n, g} g^{-1} \\
\Leftrightarrow N=\bigcup_{n \in N} \underbrace{\bigcup_{g \in G}\left\{g m_{n, g} g^{-1}\right\}}_{\text {conjugacy class of } n} \\
\Leftrightarrow N=\bigcup_{n \in N}[n],
\end{array}
$

If conversely $N$ is a subgroup of group $G$ that satisfies $N=\bigcup_{n \in N}[n]$ then it is immediate that $g n g^{-1} \in N$ for every $n \in N$ and $g \in G.$$\square$

## 4.

$\rightarrow$: For $G$, we have $\forall w\in G,w^{3}=1,$ thus $a c a^{-1} c^{-1}=$ $a^{2} b a^{2} b^{2} a^{2} b a b^{2} a^{2}=$ $\left(a^{2} b\right)^{2} b a(a b)^{2} b a^{2}=$ $b(b a)^{2} b\left(b a^{2}\right)^{2}=$ $b a^{2} b^{2} b a b^{2}=1$ $\text { so } a c=c a, $ $\text { and similarly } b c=c b .$ $ \text { Also, we have } c b a=a b, $ $\text { so } b a=c^{-1} a b=a b c^{2} \text { . }$

By the way, any word in $G$ can be written in the form $a^{i} b^{j} c^{k}$ with $i, j, k \in\{0,1,2\}$, which means that $G$ is finite with $|G| \leq 27$. To get equality, note that the Heisenberg group $H$ on $\mathbb{F}_{3}$ is generated by two elements and every non-identity element has order 3 . This means that $H$ is some quotient of $G,$ hence $|G| \geq|H|=27$.

$\leftarrow$:  $\text { Write }(z_1, z_3 ; z_2)=\left(\begin{array}{lll}
1 & z_1 & z_2 \\
& 1 & z_3 \\
& & 1
\end{array}\right)$

it suffices to check that $(z_1, z_3 ; z_2)(x, z ; y)^{-1} \in G .$ But $(x, z ; y)^{-1}=(-x,-z ; x z-y)$ and $(z_1, z_3 ; z_2)(-x,-z ; x z-y)=(z_1-x, z_3-z ; z_2-c z+x z-y) \in G$.$\square$

